examples/lowparse/LowParse.SLow.Combinators.fst
@@ -14,18 +14,18 @@ let parse32_ret
 : Tot (parser32 (parse_ret x))
 = (fun input -> ((Some (x, 0ul)) <: (res: option (t * U32.t) { parser32_correct (parse_ret x) input res } )))
 
-// inline_for_extraction
+inline_for_extraction
 let parse32_and_then
   (#k: parser_kind)
   (#t:Type)
-  (p:parser k t)
+  (#p:parser k t)
   (p32: parser32 p)
   (#k': parser_kind)
   (#t':Type)
   (p': (t -> Tot (parser k' t')))
   (u: unit { and_then_cases_injective p' } )
   (p32' : ((x: t) -> Tot (parser32 (p' x))))
-: GTot (parser32 (p `and_then` p')) // we should not use this combinator
+: Tot (parser32 (p `and_then` p'))
 = fun (input: bytes32) ->
   ((match p32 input with
   | Some (v, l) ->
@@ -72,14 +72,14 @@ inline_for_extraction
 let serialize32_nondep_then
   (#k1: parser_kind)
   (#t1: Type0)
-  (p1: parser k1 t1)
-  (s1: serializer p1)
+  (#p1: parser k1 t1)
+  (#s1: serializer p1)
   (s1' : serializer32 s1)
   (u: unit { k1.parser_kind_subkind == Some ParserStrong } )
   (#k2: parser_kind)
   (#t2: Type0)
-  (p2: parser k2 t2)
-  (s2: serializer p2)
+  (#p2: parser k2 t2)
+  (#s2: serializer p2)
   (s2' : serializer32 s2)
   (u' : unit {
     serialize32_kind_precond k1 k2
@@ -160,3 +160,42 @@ let serialize32_filter
   (f: (t -> GTot bool))
 : Tot (serializer32 #_ #_ #(parse_filter p f) (serialize_filter s f))
 = fun (input: t { f input == true } ) -> s32 input
+
+inline_for_extraction
+let make_constant_size_parser32
+  (sz: nat)
+  (sz' : U32.t { U32.v sz' == sz } )
+  (#t: Type0)
+  (f: ((s: bytes {Seq.length s == sz}) -> GTot (option t)) {
+    make_constant_size_parser_precond sz t f
+  } )
+  (f' : ((s: B32.lbytes sz) -> Tot (y: option t { y == f (B32.reveal s) } )))
+: Tot (parser32 (make_constant_size_parser sz t f))
+= fun (input: bytes32) -> ((
+    if U32.lt (B32.len input) sz'
+    then None
+    else begin
+      let s' = B32.slice input 0ul sz' in
+      match f' s' with
+      | None -> None
+      | Some v -> Some (v, sz')
+    end
+  ) <: (res: option (t * U32.t) { parser32_correct (make_constant_size_parser sz t f) input res } ))
+
+inline_for_extraction
+let make_total_constant_size_parser32
+  (sz: nat)
+  (sz' : U32.t { U32.v sz' == sz } )
+  (#t: Type0)
+  (f: ((s: bytes {Seq.length s == sz}) -> GTot (t)) {
+    make_total_constant_size_parser_precond sz t f
+  } )
+  (f' : ((s: B32.lbytes sz) -> Tot (y: t { y == f (B32.reveal s) } )))
+: Tot (parser32 (make_total_constant_size_parser sz t f))
+= fun (input: bytes32) -> ((
+    if U32.lt (B32.len input) sz'
+    then None
+    else
+      let s' = B32.slice input 0ul sz' in
+      Some (f' s', sz')
+  ) <: (res: option (t * U32.t) { parser32_correct (make_total_constant_size_parser sz t f) input res } ))
